@prefix owl: <http://www.w3.org/2002/07/owl#> .
@prefix ms: <http://github.com/usalu/semio/raw/main/src/schema/linkeddata/metasemio.ttl#> .
@prefix rdf: <http://www.w3.org/1999/02/22-rdf-syntax-ns#> .
@prefix rdfs: <http://www.w3.org/2000/01/rdf-schema#> .
@prefix se: <http://github.com/usalu/semio/raw/main/src/schema/linkeddata/semio.ttl#> .
@prefix sh: <http://www.w3.org/ns/shacl#> .
@prefix xsd: <http://www.w3.org/2001/XMLSchema#> .

se:
  a owl:Ontology ;
  rdfs:label "semio Vocabulary"@en ;
	rdfs:comment "This vocabulary defines terms for the application file format of semio.\nYou can find out more about semio on: http://github.com/usalu/semio."@en ;
	sh:declare [
		sh:prefix "se" ;
		sh:namespace "http://github.com/usalu/semio/raw/main/src/schema/linkeddata/metasemio.ttl"^^xsd:anyURI ;
	] ;
  sh:suggestedShapesGraph <http://www.w3.org/ns/shacl-shacl#> .
  owl:versionInfo "A meta schema for semio. It contains the shapes of a valid meta schema."@en ;
  ms:version "1"
.
se:Repository
  a rdfs:Class ;
  rdfs:subClassOf rdfs:Resource ;
  a sh:NodeShape ;
  sh:property [
    sh:path se:uri ;
    sh:datatype xsd:anyURI ;
    sh:minCount 1 ;
    sh:maxCount 1 ;
    sh:order 0 ;
  ]
  sh:property [
    sh:path se:layouts ;
    sh:class se:Layout ;
    sh:order 1 ;
  ]
.
se:Artifact
  a rdfs:Class ;
  rdfs:subClassOf rdfs:Resource ;
  a sh:NodeShape ;
  rdfs:label "Artifact" ;
  rdfs:comment "ğŸ“ Artifact (art/A) is anything that is produced by human or a computer." ;
  ms:abbreviation "art" ;
  ms:logogram "A" ;
  ms:symbol "ğŸ“" ;
  ms:package se:Model ;
.
se:Delineation
  a rdfs:Class ;
  rdfs:subClassOf se:Characterization ;
  a sh:NodeShape ;
  rdfs:label "Delineation" ;
  rdfs:comment "ğŸ–‹ï¸ Delineation (dln/Dl) is anything that decouples something complex." ;
  ms:abbreviation "dln" ;
  ms:logogram "Dl" ;
  ms:symbol "ğŸ–‹ï¸" ;
  ms:package se:Model ;
  sh:property [
    sh:path se:symbol ;
    sh:datatype xsd:string ;
    sh:minCount 1 ;
    sh:order 0 ;
  ]
.
se:Layout
  a rdfs:Class ;
  rdfs:subClassOf se:Delineation ;
  a sh:NodeShape ;
  rdfs:label "Layout" ;
  rdfs:comment "ğŸ–§ Layout (lyt/L) is a graph of sobjects (nodes) and attractions (slightly directed edges)." ;
  ms:abbreviation "lyt" ;
  ms:logogram "L" ;
  ms:symbol "ğŸ–§" ;
  ms:package se:Model ;
  sh:property [
    sh:path se:sobjects ;
    sh:class se:Sobject ;
    sh:minCount 1 ;
    sh:order 0 ;
  ]
.
se:Sobject
  a rdfs:Class ;
  rdfs:subClassOf se:Delineation ;
  a sh:NodeShape ;
  rdfs:label "Sobject" ;
  rdfs:comment "ğŸ›ˆ Sobject (sbj/S) is the semantic description of an object." ;
  ms:abbreviation "sbj" ;
  ms:logogram "S" ;
  ms:symbol "ğŸ›ˆ" ;
  ms:package se:Model ;
.